div attempt

Computability/RecursiveInTheorems.lean
@@ -4,7 +4,6 @@ import Mathlib.Data.PFun
 import Mathlib.Data.Nat.Dist
 
 open Classical
--- open Computability
 open Nat.RecursiveIn.Code
 
 variable {α:Type*} {β:Type*} {σ:Type*}
@@ -12,6 +11,7 @@ variable [Primcodable α] [Primcodable β] [Primcodable σ]
 
 @[simp] abbrev Nat.l (n:ℕ) := n.unpair.1
 @[simp] abbrev Nat.r (n:ℕ) := n.unpair.2
+@[simp] abbrev Nat.fzero:ℕ→ℕ:=λ_↦0
 
 namespace Nat.RecursiveIn.Code.nc_to_nn
 @[coe] protected def lift (f:ℕ→Code) : ℕ→ℕ := fun x => encodeCode (f x)
@@ -272,9 +272,9 @@ theorem prim_evaln₁:Nat.PrimrecIn O (evaln₁ O) := by
   apply _root_.PrimrecIn.comp evaln_prim h2
 
 
-theorem exists_code_for_eval₁:∃ c:ℕ, eval O c = eval₁ O := by
-  apply (exists_code_nat.mp)
-  exact rec_eval₁
+-- theorem exists_code_for_eval₁:∃ c:ℕ, eval O c = eval₁ O := by
+--   apply (exists_code_nat.mp)
+--   exact rec_eval₁
 
 theorem Nat.RecursiveIn.evalRecInO' {O} {f:ℕ→.ℕ} (h:Nat.RecursiveIn O f):Nat.RecursiveIn O (fun x => (f x) >>= (eval₁ O)) := by
   simp only [Part.bind_eq_bind]
@@ -299,220 +299,32 @@ end Nat.RecursiveIn.Code
 
 
 
-section id
-namespace Nat.RecursiveIn.Code
-def c_id := left.pair right
-@[simp] theorem c_id_ev_pr:code_prim c_id := by unfold c_id; repeat constructor
-@[simp] theorem c_id_evp:eval_prim O c_id n= n := by simp [c_id,eval_prim]
--- @[simp] theorem c_id_ev:eval O c_id n= n := by
-  -- #check @eval_prim_eq_eval c_id O c_id_ev_pr
-  -- apply (@eval_prim_eq_eval c_id O c_id_ev_pr)
-end Nat.RecursiveIn.Code
--- theorem Nat.PrimrecIn.id:Nat.PrimrecIn O Nat.id := by ...
--- theorem Nat.Primrec.id:Nat.Primrec Nat.id := by ...
-end id
-section const
-namespace Nat.RecursiveIn.Code
-def c_const:ℕ→Code
-| 0 => zero
-| n+1 => comp succ (c_const n)
-@[simp] theorem c_const_ev_pr:code_prim (c_const n) := by
-  induction n
-  · unfold c_const; exact code_prim.zero
-  · unfold c_const
-    expose_names
-    exact code_prim.comp code_prim.succ h
-@[simp] theorem c_const_ev: ∀ n m, eval_prim O (c_const n) m = n
-| 0, _ => rfl
-| n+1, m => by simp! [c_const_ev n m]
-end Nat.RecursiveIn.Code
--- theorem Nat.PrimrecIn.const:Nat.PrimrecIn O Nat.const := by ...
--- theorem Nat.Primrec.const:Nat.Primrec Nat.const := by ...
-end const
-
-section sgsg'
-/-- The signum function on naturals.  -/
-@[simp] def Nat.sg := fun x => if x=0 then 0 else 1
-/-- Maps zero to 1 and non-zero natural numbers to 0. This is the inverse of `Nat.sg` for boolean-like computations. -/
-@[simp] def Nat.sg' := fun x => if x=0 then 1 else 0
-namespace Nat.RecursiveIn.Code
-def c_sg := comp (prec zero (((c_const 1).comp left).comp left)) (pair zero c_id)
-@[simp] theorem c_sg_ev_pr:code_prim c_sg := by unfold c_sg; repeat constructor
-@[simp] theorem c_sg_evp:eval_prim O c_sg = Nat.sg := by
-  simp [c_sg,eval_prim]
-  funext n; induction n with
-  | zero => exact rfl
-  | succ n _ => simp
-@[simp] theorem c_sg_ev : eval O c_sg = Nat.sg := by rw [← eval_prim_eq_eval c_sg_ev_pr]; simp only [c_sg_evp]
-def c_sg' := comp (prec (c_const 1) (((zero).comp left).comp left)) (pair zero c_id)
-@[simp] theorem c_sg'_ev_pr:code_prim c_sg' := by unfold c_sg'; repeat constructor
-@[simp] theorem c_sg'_evp:eval_prim O c_sg' = Nat.sg' := by
-  simp [c_sg',eval_prim]
-  funext n; induction n with
-  | zero => exact rfl
-  | succ n _ => simp
-@[simp] theorem c_sg'_ev : eval O c_sg' = Nat.sg' := by rw [← eval_prim_eq_eval c_sg'_ev_pr]; simp only [c_sg'_evp]
-end Nat.RecursiveIn.Code
-theorem Nat.PrimrecIn.sg:Nat.PrimrecIn O Nat.sg := by rw [←c_sg_evp]; apply code_prim_prop c_sg_ev_pr
-theorem Nat.PrimrecIn.sg':Nat.PrimrecIn O Nat.sg' := by rw [←c_sg'_evp]; apply code_prim_prop c_sg'_ev_pr
-theorem Nat.Primrec.sg:Nat.Primrec Nat.sg := by exact PrimrecIn.PrimrecIn_Empty PrimrecIn.sg
-theorem Nat.Primrec.sg':Nat.Primrec Nat.sg' := by exact PrimrecIn.PrimrecIn_Empty PrimrecIn.sg'
-end sgsg'
-
-
-section add
-namespace Nat.RecursiveIn.Code
-def c_add := (prec c_id ((succ.comp right).comp right))
-@[simp] theorem c_add_ev_pr:code_prim c_add := by unfold c_add; repeat constructor
-@[simp] theorem c_add_evp:eval_prim O c_add = unpaired Nat.add := by
-  simp [c_add,eval_prim]
-  funext n;
-  simp [unpaired]
-  induction (unpair n).2 with
-  | zero => exact rfl
-  | succ n h => exact Nat.add_left_inj.mpr h
-@[simp] theorem c_add_ev:eval O c_add = unpaired Nat.add := by rw [← eval_prim_eq_eval c_add_ev_pr]; simp only [c_add_evp]
-end Nat.RecursiveIn.Code
--- theorem Nat.PrimrecIn.add:Nat.PrimrecIn O Nat.add := by ...
--- theorem Nat.Primrec.add:Nat.Primrec Nat.add := by ...
-end add
-section mul
-namespace Nat.RecursiveIn.Code
-def c_mul := prec zero (c_add.comp (pair left (right.comp right)))
-@[simp] theorem c_mul_ev_pr:code_prim c_mul := by unfold c_mul; repeat constructor
-@[simp] theorem c_mul_evp:eval_prim O c_mul = unpaired Nat.mul := by
-  simp [c_mul,eval_prim]
-  funext n;
-  simp [unpaired]
-  induction (unpair n).2 with
-  | zero => exact rfl
-  | succ n h =>
-    simp [*, mul_succ];
-    (expose_names; exact Nat.add_comm (unpair n_1).1 ((unpair n_1).1 * n))
-@[simp] theorem c_mul_ev:eval O c_mul = unpaired Nat.mul := by rw [← eval_prim_eq_eval c_mul_ev_pr]; simp only [c_mul_evp]
-end Nat.RecursiveIn.Code
--- theorem Nat.PrimrecIn.mul:Nat.PrimrecIn O Nat.mul := by ...
--- theorem Nat.Primrec.mul:Nat.Primrec Nat.mul := by ...
-end mul
-
-section prec1
-namespace Nat.RecursiveIn.Code
-def c_prec1 (m) (cf:Code) := ((prec (c_const m) (cf.comp right)).comp (zero.pair c_id))
-@[simp] theorem c_prec1_ev_pr (hcf:code_prim cf) : code_prim (@c_prec1 m cf) := by
-  unfold c_prec1;
-  repeat constructor
-  simp
-  repeat constructor
-  exact hcf
-  repeat constructor
-@[simp] theorem c_prec1_ev : eval_prim O (c_prec1 m cf) = (fun n => n.rec m fun y IH => eval_prim O cf <| Nat.pair y IH) := by simp [c_prec1,eval_prim]
-end Nat.RecursiveIn.Code
--- theorem Nat.PrimrecIn.prec1:Nat.PrimrecIn O Nat.prec1 := by ...
--- theorem Nat.Primrec.prec1:Nat.Primrec Nat.prec1 := by ...
-end prec1
-section casesOn1
-namespace Nat.RecursiveIn.Code
-def c_casesOn1 (m) (cf:Code) := @c_prec1 m (cf.comp left)
--- theorem c_casesOn1_ev_pr:code_prim (@c_casesOn1 a b) := by unfold c_casesOn1; repeat constructor;
-@[simp] theorem c_casesOn1_ev : eval_prim O (@c_casesOn1 m cf) = (Nat.casesOn · m (eval_prim O cf)) := by simp [c_casesOn1,eval_prim]
-end Nat.RecursiveIn.Code
--- theorem Nat.PrimrecIn.casesOn1:Nat.PrimrecIn O Nat.casesOn1 := by ...
--- theorem Nat.Primrec.casesOn1:Nat.Primrec Nat.casesOn1 := by ...
-end casesOn1
-
-section pred
-namespace Nat.RecursiveIn.Code
-def c_pred := (c_casesOn1 0 c_id)
-@[simp] theorem c_pred_ev_pr:code_prim c_pred := by unfold c_pred; repeat constructor
-@[simp] theorem c_pred_evp:eval_prim O c_pred = Nat.pred := by
-  simp [c_pred,eval_prim]
-  funext n;
-  cases n <;> simp [*]
-@[simp] theorem c_pred_ev:eval O c_pred = Nat.pred := by rw [← eval_prim_eq_eval c_pred_ev_pr]; simp only [c_pred_evp]
-end Nat.RecursiveIn.Code
--- theorem Nat.PrimrecIn.pred:Nat.PrimrecIn O Nat.pred := by ...
--- theorem Nat.Primrec.pred:Nat.Primrec Nat.pred := by ...
-end pred
-section sub
-namespace Nat.RecursiveIn.Code
-def c_sub := prec c_id ((c_pred.comp right).comp right)
-@[simp] theorem c_sub_ev_pr:code_prim c_sub := by unfold c_sub; repeat constructor
-@[simp] theorem c_sub_evp:eval_prim O c_sub = unpaired Nat.sub := by
-  simp [c_sub,eval_prim]
-  funext n;
-  simp [unpaired]
-  induction (unpair n).2 with
-  | zero => exact rfl
-  | succ n h =>
-    simp [*, Nat.sub_add_eq];
-@[simp] theorem c_sub_ev:eval O c_sub = unpaired Nat.sub := by rw [← eval_prim_eq_eval c_sub_ev_pr]; simp only [c_sub_evp]
-end Nat.RecursiveIn.Code
--- theorem Nat.PrimrecIn.sub:Nat.PrimrecIn O Nat.sub := by ...
--- theorem Nat.Primrec.sub:Nat.Primrec Nat.sub := by ...
-end sub
-section dist
-namespace Nat.RecursiveIn.Code
-def c_dist := c_add.comp (pair c_sub (c_sub.comp (pair right left)))
-@[simp] theorem c_dist_ev_pr:code_prim c_dist := by unfold c_dist; repeat constructor
-@[simp] theorem c_dist_evp:eval_prim O c_dist = unpaired Nat.dist := by simp [c_dist,eval_prim]; exact rfl
-@[simp] theorem c_dist_ev:eval O c_dist = unpaired Nat.dist := by rw [← eval_prim_eq_eval c_dist_ev_pr]; simp only [c_dist_evp]
-end Nat.RecursiveIn.Code
--- theorem Nat.PrimrecIn.dist:Nat.PrimrecIn O Nat.dist := by ...
--- theorem Nat.Primrec.dist:Nat.Primrec Nat.dist := by ...
-end dist
-@[simp] theorem eq_zero_iff_dist_zero {a b:ℕ} : a.dist b = 0 ↔ a=b := by
-  constructor
-  · exact fun a_1 ↦ Nat.eq_of_dist_eq_zero a_1
-  · exact fun a_1 ↦ Nat.dist_eq_zero a_1
-theorem sgdist_eq_ifeq {a b:ℕ} : (if a.dist b = 0 then 0 else 1) = (if a=b then 0 else 1) := by
-  simp only [eq_zero_iff_dist_zero]
-
-section if_eq'
-namespace Nat.RecursiveIn.Code
-def c_if_eq' := c_sg.comp c_dist
-@[simp] theorem c_if_eq'_ev_pr:code_prim c_if_eq' := by unfold c_if_eq'; repeat constructor
-@[simp] theorem c_if_eq'_evp:eval_prim O c_if_eq' = fun ab => if ab.l=ab.r then 0 else 1 := by simp [c_if_eq',eval_prim];
-@[simp] theorem c_if_eq'_ev:eval O c_if_eq' = fun ab => if ab.l=ab.r then 0 else 1 := by rw [← eval_prim_eq_eval c_if_eq'_ev_pr]; simp only [c_if_eq'_evp]; simp; funext xs; exact apply_ite Part.some ((unpair xs).1 = (unpair xs).2) 0 1
-end Nat.RecursiveIn.Code
--- theorem Nat.PrimrecIn.if_eq':Nat.PrimrecIn O Nat.if_eq' := by ...
--- theorem Nat.Primrec.if_eq':Nat.Primrec Nat.if_eq' := by ...
-end if_eq'
 
 
 
 
 
-/-- Given a total choice function `c`, returns `a` or `b` conditioning on whether `c x=0`. -/
-theorem Nat.RecursiveIn.ifz1 {O:ℕ→ℕ} {c:ℕ→ℕ} (hc:Nat.RecursiveIn O c): Nat.RecursiveIn O (fun x => if (c x=0) then (a:ℕ) else (b:ℕ):ℕ→ℕ) := by
-  let construction := fun x =>
-    Nat.add
-    (Nat.mul b (Nat.sg (c x)))
-    (Nat.mul a (Nat.sg' (c x)))
-  have consRecin:Nat.RecursiveIn O construction := by
-    simp only [construction]
-    apply Nat.RecursiveIn.totalComp₂
-    · apply of_primrec Nat.Primrec.add
-    · apply Nat.RecursiveIn.totalComp₂
-      · apply of_primrec Nat.Primrec.mul
-      · apply of_primrec (Nat.Primrec.const b)
-      · apply Nat.RecursiveIn.totalComp'
-        · exact of_primrec Nat.Primrec.sg
-        · exact hc
-    · apply Nat.RecursiveIn.totalComp₂
-      · apply of_primrec Nat.Primrec.mul
-      · apply of_primrec (Nat.Primrec.const a)
-      · apply Nat.RecursiveIn.totalComp'
-        · exact of_primrec Nat.Primrec.sg'
-        · exact hc
-  have consEq: (fun x => if (c x=0) then (a:ℕ) else (b:ℕ):ℕ→ℕ) = construction := by
-    simp [construction]
-    funext xs
-    cases Classical.em (c xs = 0) with -- do i really need classical.em here?
-      | inl h => simp [h]
-      | inr h => simp [h]
 
-  rw [consEq]
-  exact consRecin
+
+
+
+
+
+
+
+
+
+
+
+
+
+
+
+
+
+
+
+
 
 
 
@@ -530,43 +342,3 @@ lemma Nat.Primrec.pair_proj:Nat.Primrec (Nat.pair x) := by
   refine Primrec.nat_iff.mp ?_
   apply Primrec.projection
   exact Primrec₂.natPair
-
-
-
-
-theorem Nat.RecursiveIn.ite {O:ℕ→ℕ} {f g:ℕ→.ℕ} {c:ℕ→ℕ} (hc:Nat.RecursiveIn O c) (hf:Nat.RecursiveIn O f) (hg:Nat.RecursiveIn O g):Nat.RecursiveIn O fun a => if (c a=0) then (f a) else (g a) := by
-    have exists_index_for_f:∃ c:ℕ, eval O c = f := by exact exists_code_nat.mp hf
-    have exists_index_for_g:∃ c:ℕ, eval O c = g := by exact exists_code_nat.mp hg
-    rcases exists_index_for_f with ⟨index_f,index_f_is_f⟩
-    rcases exists_index_for_g with ⟨index_g,index_g_is_g⟩
-
-    have main2:(fun a => if (c a=0) then (f a) else (g a)) = fun a => Nat.pair (if c a=0 then (index_f) else (index_g)) a >>= eval₁ O := by
-      funext xs
-      cases Classical.em (c xs = 0) with
-      | inl h =>
-        simp only [h, ↓reduceIte, Part.coe_some, Part.bind_eq_bind, Part.bind_some, eval₁, Nat.unpair_pair]
-        exact congrFun (_root_.id (Eq.symm index_f_is_f)) xs
-      | inr h =>
-        simp only [h, ↓reduceIte, Part.coe_some, Part.bind_eq_bind, Part.bind_some, eval₁, Nat.unpair_pair]
-        exact congrFun (_root_.id (Eq.symm index_g_is_g)) xs
-    rw [main2]
-
-
-    apply Nat.RecursiveIn.evalRecInO'
-    apply Nat.RecursiveIn.someTotal
-
-    rw [Nat.RecursiveIn.pair']
-
-    apply Nat.RecursiveIn.pair
-    · simp only [Part.coe_some]
-      apply Nat.RecursiveIn.ifz1
-      exact hc
-    exact id
-
--- for code_ifeq
-
-
-
-/--`[code_if_eval_eq c](x)=0 if x.1=x.2 else 1`-/
-def code_if_eq:ℕ→ℕ := fun x => 0
-theorem code_if_eq_prop:eval O (code_if_eq e) ab = if (Nat.succ ab.l.r=eval O e (Nat.pair ab.l.l ab.r)) then 0 else 1 := by sorry
