Computability/Constructions.lean
@@ -1,0 +1,485 @@
+import Computability.RecursiveInTheorems
+
+open Nat.RecursiveIn.Code
+
+
+
+section id
+namespace Nat.RecursiveIn.Code
+def c_id := left.pair right
+@[simp] theorem c_id_ev_pr:code_prim c_id := by unfold c_id; repeat constructor
+@[simp] theorem c_id_evp:eval_prim O c_id n= n := by simp [c_id,eval_prim]
+@[simp] theorem c_id_ev:eval O c_id n = n := by simp [c_id,eval,Seq.seq]
+  -- #check @eval_prim_eq_eval c_id O c_id_ev_pr
+  -- apply (@eval_prim_eq_eval c_id O c_id_ev_pr)
+end Nat.RecursiveIn.Code
+-- theorem Nat.PrimrecIn.id:Nat.PrimrecIn O Nat.id := by ...
+-- theorem Nat.Primrec.id:Nat.Primrec Nat.id := by ...
+end id
+section const
+namespace Nat.RecursiveIn.Code
+def c_const:ℕ→Code
+| 0 => zero
+| n+1 => comp succ (c_const n)
+@[simp] theorem c_const_ev_pr:code_prim (c_const n) := by
+  induction n
+  · unfold c_const; exact code_prim.zero
+  · unfold c_const
+    expose_names
+    exact code_prim.comp code_prim.succ h
+@[simp] theorem c_const_evp: ∀ n m, eval_prim O (c_const n) m = n
+| 0, _ => rfl
+| n+1, m => by simp! [c_const_evp n m]
+end Nat.RecursiveIn.Code
+-- theorem Nat.PrimrecIn.const:Nat.PrimrecIn O Nat.const := by ...
+-- theorem Nat.Primrec.const:Nat.Primrec Nat.const := by ...
+end const
+section curry
+namespace Nat.RecursiveIn.Code
+def c_curry (c : Code) (n : ℕ) : Code := comp c (pair (c_const n) c_id)
+theorem _id_eq_c_id : c_id = Code.id := by simp [c_id,Code.id]
+theorem _const_eq_c_const : c_const = Code.const := by
+  funext n;
+  unfold c_const
+  unfold Code.const
+  induction n
+  · exact rfl
+  · simp
+    unfold c_const
+    unfold Code.const
+    expose_names
+    exact h
+theorem _curry_eq_c_curry : c_curry = curry := by
+  unfold c_curry
+  unfold curry
+  rw [_id_eq_c_id]
+  rw [_const_eq_c_const]
+-- @[simp] theorem c_curry_ev_pr:code_prim (c_curry c n) := by
+@[simp] theorem c_curry_evp: eval_prim O (c_curry c n) x = eval_prim O c (Nat.pair n x) := by simp [c_curry,eval_prim]
+@[simp] theorem c_curry_ev: eval O (c_curry c n) x = eval O c (Nat.pair n x) := by rw [_curry_eq_c_curry]; exact eval_curry c n x
+
+end Nat.RecursiveIn.Code
+-- theorem Nat.PrimrecIn.curry:Nat.PrimrecIn O Nat.curry := by ...
+-- theorem Nat.Primrec.curry:Nat.Primrec Nat.curry := by ...
+end curry
+
+section sgsg'
+/-- The signum function on naturals.  -/
+@[simp] def Nat.sg := fun x => if x=0 then 0 else 1
+/-- Maps zero to 1 and non-zero natural numbers to 0. This is the inverse of `Nat.sg` for boolean-like computations. -/
+@[simp] def Nat.sg' := fun x => if x=0 then 1 else 0
+namespace Nat.RecursiveIn.Code
+def c_sg := comp (prec zero (((c_const 1).comp left).comp left)) (pair zero c_id)
+@[simp] theorem c_sg_ev_pr:code_prim c_sg := by unfold c_sg; repeat constructor
+@[simp] theorem c_sg_evp:eval_prim O c_sg = Nat.sg := by
+  simp [c_sg,eval_prim]
+  funext n; induction n with
+  | zero => exact rfl
+  | succ n _ => simp
+@[simp] theorem c_sg_ev : eval O c_sg = Nat.sg := by rw [← eval_prim_eq_eval c_sg_ev_pr]; simp only [c_sg_evp]
+def c_sg' := comp (prec (c_const 1) (((zero).comp left).comp left)) (pair zero c_id)
+@[simp] theorem c_sg'_ev_pr:code_prim c_sg' := by unfold c_sg'; repeat constructor
+@[simp] theorem c_sg'_evp:eval_prim O c_sg' = Nat.sg' := by
+  simp [c_sg',eval_prim]
+  funext n; induction n with
+  | zero => exact rfl
+  | succ n _ => simp
+@[simp] theorem c_sg'_ev : eval O c_sg' = Nat.sg' := by rw [← eval_prim_eq_eval c_sg'_ev_pr]; simp only [c_sg'_evp]
+end Nat.RecursiveIn.Code
+theorem Nat.PrimrecIn.sg:Nat.PrimrecIn O Nat.sg := by rw [←c_sg_evp]; apply code_prim_prop c_sg_ev_pr
+theorem Nat.PrimrecIn.sg':Nat.PrimrecIn O Nat.sg' := by rw [←c_sg'_evp]; apply code_prim_prop c_sg'_ev_pr
+theorem Nat.Primrec.sg:Nat.Primrec Nat.sg := by exact PrimrecIn.PrimrecIn_Empty PrimrecIn.sg
+theorem Nat.Primrec.sg':Nat.Primrec Nat.sg' := by exact PrimrecIn.PrimrecIn_Empty PrimrecIn.sg'
+end sgsg'
+
+
+section add
+namespace Nat.RecursiveIn.Code
+def c_add := (prec c_id ((succ.comp right).comp right))
+@[simp] theorem c_add_ev_pr:code_prim c_add := by unfold c_add; repeat constructor
+@[simp] theorem c_add_evp:eval_prim O c_add = unpaired Nat.add := by
+  simp [c_add,eval_prim]
+  funext n;
+  simp [unpaired]
+  induction (unpair n).2 with
+  | zero => exact rfl
+  | succ n h => exact Nat.add_left_inj.mpr h
+@[simp] theorem c_add_ev:eval O c_add = unpaired Nat.add := by rw [← eval_prim_eq_eval c_add_ev_pr]; simp only [c_add_evp]
+end Nat.RecursiveIn.Code
+-- theorem Nat.PrimrecIn.add:Nat.PrimrecIn O Nat.add := by ...
+-- theorem Nat.Primrec.add:Nat.Primrec Nat.add := by ...
+end add
+section mul
+namespace Nat.RecursiveIn.Code
+def c_mul := prec zero (c_add.comp (pair left (right.comp right)))
+@[simp] theorem c_mul_ev_pr:code_prim c_mul := by unfold c_mul; repeat constructor
+@[simp] theorem c_mul_evp:eval_prim O c_mul = unpaired Nat.mul := by
+  simp [c_mul,eval_prim]
+  funext n;
+  simp [unpaired]
+  induction (unpair n).2 with
+  | zero => exact rfl
+  | succ n h =>
+    simp [*, mul_succ];
+    (expose_names; exact Nat.add_comm (unpair n_1).1 ((unpair n_1).1 * n))
+@[simp] theorem c_mul_ev:eval O c_mul = unpaired Nat.mul := by rw [← eval_prim_eq_eval c_mul_ev_pr]; simp only [c_mul_evp]
+end Nat.RecursiveIn.Code
+-- theorem Nat.PrimrecIn.mul:Nat.PrimrecIn O Nat.mul := by ...
+-- theorem Nat.Primrec.mul:Nat.Primrec Nat.mul := by ...
+end mul
+section pow
+namespace Nat.RecursiveIn.Code
+def c_pow := prec (c_const 1) (c_mul.comp (pair (right.comp right) left))
+@[simp] theorem c_pow_ev_pr:code_prim c_pow := by unfold c_pow; repeat constructor
+@[simp] theorem c_pow_evp:eval_prim O c_pow = unpaired Nat.pow := by
+  simp [c_pow,eval_prim]
+  funext n;
+  simp [unpaired]
+
+  induction (unpair n).2 with
+  | zero => exact rfl
+  | succ n h => simp [*, pow_succ];
+@[simp] theorem c_pow_ev:eval O c_pow = unpaired Nat.pow := by rw [← eval_prim_eq_eval c_pow_ev_pr]; simp only [c_pow_evp]
+end Nat.RecursiveIn.Code
+-- theorem Nat.PrimrecIn.pow:Nat.PrimrecIn O Nat.pow := by ...
+-- theorem Nat.Primrec.pow:Nat.Primrec Nat.pow := by ...
+end pow
+
+section prec1
+namespace Nat.RecursiveIn.Code
+def c_prec1 (m) (cf:Code) := ((prec (c_const m) (cf.comp right)).comp (zero.pair c_id))
+@[simp] theorem c_prec1_ev_pr (hcf:code_prim cf) : code_prim (@c_prec1 m cf) := by
+  unfold c_prec1;
+  repeat constructor
+  simp
+  repeat constructor
+  exact hcf
+  repeat constructor
+@[simp] theorem c_prec1_ev : eval_prim O (c_prec1 m cf) = (fun n => n.rec m fun y IH => eval_prim O cf <| Nat.pair y IH) := by simp [c_prec1,eval_prim]
+end Nat.RecursiveIn.Code
+-- theorem Nat.PrimrecIn.prec1:Nat.PrimrecIn O Nat.prec1 := by ...
+-- theorem Nat.Primrec.prec1:Nat.Primrec Nat.prec1 := by ...
+end prec1
+section casesOn1
+namespace Nat.RecursiveIn.Code
+def c_casesOn1 (m) (cf:Code) := @c_prec1 m (cf.comp left)
+-- theorem c_casesOn1_ev_pr:code_prim (@c_casesOn1 a b) := by unfold c_casesOn1; repeat constructor;
+@[simp] theorem c_casesOn1_ev : eval_prim O (@c_casesOn1 m cf) = (Nat.casesOn · m (eval_prim O cf)) := by simp [c_casesOn1,eval_prim]
+end Nat.RecursiveIn.Code
+-- theorem Nat.PrimrecIn.casesOn1:Nat.PrimrecIn O Nat.casesOn1 := by ...
+-- theorem Nat.Primrec.casesOn1:Nat.Primrec Nat.casesOn1 := by ...
+end casesOn1
+
+section pred
+namespace Nat.RecursiveIn.Code
+def c_pred := (c_casesOn1 0 c_id)
+@[simp] theorem c_pred_ev_pr:code_prim c_pred := by unfold c_pred; repeat constructor
+@[simp] theorem c_pred_evp:eval_prim O c_pred = Nat.pred := by
+  simp [c_pred,eval_prim]
+  funext n;
+  cases n <;> simp [*]
+@[simp] theorem c_pred_ev:eval O c_pred = Nat.pred := by rw [← eval_prim_eq_eval c_pred_ev_pr]; simp only [c_pred_evp]
+end Nat.RecursiveIn.Code
+-- theorem Nat.PrimrecIn.pred:Nat.PrimrecIn O Nat.pred := by ...
+-- theorem Nat.Primrec.pred:Nat.Primrec Nat.pred := by ...
+end pred
+section sub
+namespace Nat.RecursiveIn.Code
+def c_sub := prec c_id ((c_pred.comp right).comp right)
+@[simp] theorem c_sub_ev_pr:code_prim c_sub := by unfold c_sub; repeat constructor
+@[simp] theorem c_sub_evp:eval_prim O c_sub = unpaired Nat.sub := by
+  simp [c_sub,eval_prim]
+  funext n;
+  simp [unpaired]
+  induction (unpair n).2 with
+  | zero => exact rfl
+  | succ n h =>
+    simp [*, Nat.sub_add_eq];
+@[simp] theorem c_sub_ev:eval O c_sub = unpaired Nat.sub := by rw [← eval_prim_eq_eval c_sub_ev_pr]; simp only [c_sub_evp]
+end Nat.RecursiveIn.Code
+-- theorem Nat.PrimrecIn.sub:Nat.PrimrecIn O Nat.sub := by ...
+-- theorem Nat.Primrec.sub:Nat.Primrec Nat.sub := by ...
+end sub
+section dist
+namespace Nat.RecursiveIn.Code
+def c_dist := c_add.comp (pair c_sub (c_sub.comp (pair right left)))
+@[simp] theorem c_dist_ev_pr:code_prim c_dist := by unfold c_dist; repeat constructor
+@[simp] theorem c_dist_evp:eval_prim O c_dist = unpaired Nat.dist := by simp [c_dist,eval_prim]; exact rfl
+@[simp] theorem c_dist_ev:eval O c_dist = unpaired Nat.dist := by rw [← eval_prim_eq_eval c_dist_ev_pr]; simp only [c_dist_evp]
+end Nat.RecursiveIn.Code
+-- theorem Nat.PrimrecIn.dist:Nat.PrimrecIn O Nat.dist := by ...
+-- theorem Nat.Primrec.dist:Nat.Primrec Nat.dist := by ...
+end dist
+@[simp] theorem eq_zero_iff_dist_zero {a b:ℕ} : a.dist b = 0 ↔ a=b := by
+  constructor
+  · exact fun a_1 ↦ Nat.eq_of_dist_eq_zero a_1
+  · exact fun a_1 ↦ Nat.dist_eq_zero a_1
+theorem sgdist_eq_ifeq {a b:ℕ} : (if a.dist b = 0 then 0 else 1) = (if a=b then 0 else 1) := by
+  simp only [eq_zero_iff_dist_zero]
+
+section if_eq'
+namespace Nat.RecursiveIn.Code
+def c_if_eq' := c_sg.comp c_dist
+@[simp] theorem c_if_eq'_ev_pr:code_prim c_if_eq' := by unfold c_if_eq'; repeat constructor
+@[simp] theorem c_if_eq'_evp:eval_prim O c_if_eq' = fun ab => if ab.l=ab.r then 0 else 1 := by simp [c_if_eq',eval_prim];
+@[simp] theorem c_if_eq'_ev:eval O c_if_eq' = fun ab => if ab.l=ab.r then 0 else 1 := by rw [← eval_prim_eq_eval c_if_eq'_ev_pr]; simp only [c_if_eq'_evp]; simp; funext xs; exact apply_ite Part.some ((unpair xs).1 = (unpair xs).2) 0 1
+end Nat.RecursiveIn.Code
+-- theorem Nat.PrimrecIn.if_eq':Nat.PrimrecIn O Nat.if_eq' := by ...
+-- theorem Nat.Primrec.if_eq':Nat.Primrec Nat.if_eq' := by ...
+end if_eq'
+
+
+
+
+section ef
+namespace Nat.RecursiveIn.Code
+def c_ef:ℕ→ℕ:=fun c=>(pair Nat.RecursiveIn.Code.id c)
+-- @[simp] theorem c_ef_ev_pr:code_prim $ c_ef c := by unfold c_ef; repeat constructor
+@[simp] theorem c_ef_pr_aux:Primrec (pair Nat.RecursiveIn.Code.id) := by
+  refine Primrec.projection ?_
+  apply PrimrecIn.PrimrecIn₂_iff_Primrec₂.mp
+  intro O
+  apply pair_prim
+@[simp] theorem c_ef_pr: Nat.Primrec c_ef := by
+  refine Primrec.nat_iff.mp ?_
+  apply c_ef_pr_aux
+-- @[simp] theorem c_ef_evp:eval_prim O c_ef = fun ab => if ab.l=ab.r then 0 else 1 := by simp [c_ef,eval_prim];
+theorem c_ef_ev : eval O (c_ef c) x = Nat.pair <$> x <*> (eval O c x) := by simp [c_ef,eval]
+end Nat.RecursiveIn.Code
+-- theorem Nat.PrimrecIn.ef:Nat.PrimrecIn O Nat.ef := by ...
+-- theorem Nat.Primrec.ef:Nat.Primrec Nat.ef := by ...
+theorem c_ef_ev_left (h:(eval O c x).Dom) : eval O (left.comp $ c_ef c) x = x := by
+  have h0 : (eval O c x).get h ∈ (eval O c x) := by exact Part.get_mem h
+  have h1 : eval O c x = Part.some ((eval O c x).get h) := by exact Part.get_eq_iff_eq_some.mp rfl
+
+  simp [c_ef, eval]
+  rw [h1]
+  -- should maybe define some theorem that simplfies the Nat.pair <*> business
+  simp [Seq.seq]
+  exact Part.Dom.bind h fun y ↦ Part.some x
+end ef
+
+
+
+section l_append
+def Nat.list_append (list index:ℕ):ℕ:=Nat.pair (list.l+1) $ Nat.pair list.r index
+namespace Nat.RecursiveIn.Code
+def c_l_append := pair (succ.comp $ left.comp left) (pair (right.comp left) right)
+@[simp] theorem c_l_append_ev_pr:code_prim c_l_append := by unfold c_l_append; repeat constructor
+@[simp] theorem c_l_append_evp:eval_prim O c_l_append = unpaired Nat.list_append := by unfold Nat.list_append; simp [c_l_append,eval_prim];
+@[simp] theorem c_l_append_ev:eval O c_l_append = unpaired Nat.list_append := by rw [← eval_prim_eq_eval c_l_append_ev_pr]; simp only [c_l_append_evp]
+end Nat.RecursiveIn.Code
+-- theorem Nat.PrimrecIn.l_append:Nat.PrimrecIn O Nat.l_append := by ...
+-- theorem Nat.Primrec.l_append:Nat.Primrec Nat.l_append := by ...
+end l_append
+
+
+
+
+
+section l_get_last
+def Nat.list_get_last_aux (list index:ℕ):ℕ:=
+  match index with
+  | 0 => list.r
+  | Nat.succ prev_index => (Nat.list_get_last_aux list prev_index).l
+def Nat.list_get_lastn (list index:ℕ):ℕ:=(Nat.list_get_last_aux list index).r
+def Nat.list_get_last (list:ℕ) :=list.r.r
+
+namespace Nat.RecursiveIn.Code
+def c_l_get_lastn_aux := prec right (left.comp $ right.comp right)
+@[simp] theorem c_l_get_lastn_aux_ev_pr:code_prim c_l_get_lastn_aux := by unfold c_l_get_lastn_aux; repeat constructor
+@[simp] theorem c_l_get_lastn_aux_evp:eval_prim O c_l_get_lastn_aux = unpaired Nat.list_get_last_aux := by
+  simp [c_l_get_lastn_aux,eval_prim];
+  funext n;
+  simp [unpaired]
+  induction (unpair n).2 with
+  | zero => exact rfl
+  | succ n h => exact congrArg Prod.fst (congrArg unpair h)
+@[simp] theorem c_l_get_lastn_aux_ev:eval O c_l_get_lastn_aux = unpaired Nat.list_get_last_aux := by rw [← eval_prim_eq_eval c_l_get_lastn_aux_ev_pr]; simp only [c_l_get_lastn_aux_evp];
+
+def c_l_get_lastn := right.comp c_l_get_lastn_aux
+@[simp] theorem c_l_get_lastn_ev_pr:code_prim c_l_get_lastn := by unfold c_l_get_lastn; repeat constructor
+@[simp] theorem c_l_get_lastn_evp:eval_prim O c_l_get_lastn = unpaired Nat.list_get_lastn := by
+  unfold list_get_lastn
+  simp [c_l_get_lastn,eval_prim];
+@[simp] theorem c_l_get_lastn_ev:eval O c_l_get_lastn = unpaired Nat.list_get_lastn := by rw [← eval_prim_eq_eval c_l_get_lastn_ev_pr]; simp only [c_l_get_lastn_evp];
+
+def c_l_get_last := c_l_get_lastn.comp $ pair c_id (c_const 0)
+@[simp] theorem c_l_get_last_ev_pr:code_prim c_l_get_last := by unfold c_l_get_last; repeat constructor;
+@[simp] theorem c_l_get_last_evp:eval_prim O c_l_get_last = Nat.list_get_last := by
+  unfold list_get_last
+  simp [c_l_get_last,eval_prim];
+  exact rfl
+@[simp] theorem c_l_get_last_ev:eval O c_l_get_last = Nat.list_get_last := by rw [← eval_prim_eq_eval c_l_get_last_ev_pr]; simp only [c_l_get_last_evp];
+end Nat.RecursiveIn.Code
+-- theorem Nat.PrimrecIn.l_get:Nat.PrimrecIn O Nat.l_get := by ...
+-- theorem Nat.Primrec.l_get:Nat.Primrec Nat.l_get := by ...
+end l_get_last
+
+@[simp] theorem Nat.list_get_last_append : Nat.list_get_last (Nat.list_append lst x) = x := by
+  unfold list_append
+  unfold list_get_last
+  simp
+
+
+
+section efl
+namespace Nat.RecursiveIn.Code
+def c_efl:ℕ→ℕ:=fun c=>c_l_append.comp (pair c_id c)
+@[simp] theorem c_efl_ev_pr (h:code_prim c):code_prim $ c_efl c := by
+  unfold c_efl;
+  simp
+  repeat constructor
+  exact h
+-- @[simp] theorem c_efl_pr_aux:Primrec (pair c_id) := by
+--   refine Primrec.projection ?_
+--   apply PrimrecIn.PrimrecIn₂_iff_Primrec₂.mp
+--   intro O
+--   apply pair_prim
+-- @[simp] theorem c_efl_pr: Nat.Primrec c_efl := by
+--   refine Primrec.nat_iff.mp ?_
+--   apply c_efl_pr_aux
+
+-- huh interesting, it doesn't care about c being code_prim or not.
+@[simp] theorem c_efl_evp:eval_prim O (c_efl c) x= Nat.list_append x (eval_prim O c x) := by
+  unfold list_append
+  simp [c_efl,eval_prim];
+  unfold list_append
+  simp
+@[simp] theorem c_efl_ev : eval O (c_efl c) x = Nat.list_append <$> x <*> (eval O c x) := by
+  unfold Nat.list_append
+  simp [c_efl,eval]
+  simp [Seq.seq]
+  exact Part.bind_some_eq_map x.list_append (eval O (decodeCode c) x)
+end Nat.RecursiveIn.Code
+-- theorem Nat.PrimrecIn.efl:Nat.PrimrecIn O Nat.efl := by ...
+-- theorem Nat.Primrec.efl:Nat.Primrec Nat.efl := by ...
+-- theorem c_efl_ev_left (h:(eval O c x).Dom) : eval O (left.comp $ c_efl c) x = x := by
+--   have h0 : (eval O c x).get h ∈ (eval O c x) := by exact Part.get_mem h
+--   have h1 : eval O c x = Part.some ((eval O c x).get h) := by exact Part.get_eq_iff_eq_some.mp rfl
+
+--   simp [c_efl, eval]
+--   rw [h1]
+--   -- should maybe define some theorem that simplfies the Nat.pair <*> business
+--   simp [Seq.seq]
+--   exact Part.Dom.bind h fun y ↦ Part.some x
+end efl
+
+@[simp] theorem last_efl : eval_prim O (c_l_get_last.comp (c_efl c)) = eval_prim O c := by
+  simp only [eval_prim]
+  simp
+
+
+
+def Nat.list_empty := Nat.pair 0 0
+
+section div_flip
+namespace Nat.RecursiveIn.Code
+-- def c_div_flip_aux := prec (c_const $ Nat.list_append Nat.list_empty 0) $ c_efl $ c_mul.comp $ pair (c_sg.comp $ c_sub.comp $ pair (right.comp left) left) (succ.comp (c_l_get_lastn.curry left))
+def c_div_flip_aux := c_efl $ prec (c_const 0) $ c_mul.comp $ pair (c_sg.comp $ c_sub.comp $ pair (right.comp left) left) (succ.comp (c_l_get_lastn.comp $ pair c_id left))
+def c_div_flip := c_l_get_last.comp c_div_flip_aux
+-- @[simp] theorem c_div_flip_ev_pr:code_prim c_div_flip := by unfold c_div_flip; repeat constructor
+@[simp] theorem c_div_flip_evp:eval_prim O c_div_flip = unpaired (flip ((· / ·) : ℕ → ℕ → ℕ)) := by
+  unfold c_div_flip
+  unfold c_div_flip_aux
+  simp [c_div_flip,eval_prim, c_div_flip_aux]
+  funext n;
+  simp [unpaired]
+  induction (unpair n).2 using Nat.strong_induction_on with
+  | h =>
+    expose_names
+
+
+  -- induction (unpair n).2 using Nat.strong_induction_on with
+  -- | zero => simp [flip]
+  -- | succ n h =>
+  --   simp
+  --   simp [list_append]
+
+@[simp] theorem c_div_ev:eval O c_div = unpaired Nat.div := by rw [← eval_prim_eq_eval c_div_ev_pr]; simp only [c_div_evp]
+end Nat.RecursiveIn.Code
+-- theorem Nat.PrimrecIn.div:Nat.PrimrecIn O Nat.div := by ...
+-- theorem Nat.Primrec.div:Nat.Primrec Nat.div := by ...
+end div
+
+#eval Nat.div 6 3
+#eval eval_prim Nat.fzero c_add $ Nat.pair 2 6
+-- #eval eval_prim Nat.fzero c_mul $ Nat.pair 223 6123
+-- #eval Nat.mul 223 6123
+-- #reduce eval_prim Nat.fzero c_mul $ Nat.pair 2 3
+-- #eval eval_prim Nat.fzero c_div $ Nat.pair 2 6
+
+
+
+
+
+
+
+
+
+
+
+
+
+
+
+/-- Given a total choice function `c`, returns `a` or `b` conditioning on whether `c x=0`. -/
+theorem Nat.RecursiveIn.ifz1 {O:ℕ→ℕ} {c:ℕ→ℕ} (hc:Nat.RecursiveIn O c): Nat.RecursiveIn O (fun x => if (c x=0) then (a:ℕ) else (b:ℕ):ℕ→ℕ) := by
+  let construction := fun x =>
+    Nat.add
+    (Nat.mul b (Nat.sg (c x)))
+    (Nat.mul a (Nat.sg' (c x)))
+  have consRecin:Nat.RecursiveIn O construction := by
+    simp only [construction]
+    apply Nat.RecursiveIn.totalComp₂
+    · apply of_primrec Nat.Primrec.add
+    · apply Nat.RecursiveIn.totalComp₂
+      · apply of_primrec Nat.Primrec.mul
+      · apply of_primrec (Nat.Primrec.const b)
+      · apply Nat.RecursiveIn.totalComp'
+        · exact of_primrec Nat.Primrec.sg
+        · exact hc
+    · apply Nat.RecursiveIn.totalComp₂
+      · apply of_primrec Nat.Primrec.mul
+      · apply of_primrec (Nat.Primrec.const a)
+      · apply Nat.RecursiveIn.totalComp'
+        · exact of_primrec Nat.Primrec.sg'
+        · exact hc
+  have consEq: (fun x => if (c x=0) then (a:ℕ) else (b:ℕ):ℕ→ℕ) = construction := by
+    simp [construction]
+    funext xs
+    cases Classical.em (c xs = 0) with -- do i really need classical.em here?
+      | inl h => simp [h]
+      | inr h => simp [h]
+
+  rw [consEq]
+  exact consRecin
+
+theorem Nat.RecursiveIn.ite {O:ℕ→ℕ} {f g:ℕ→.ℕ} {c:ℕ→ℕ} (hc:Nat.RecursiveIn O c) (hf:Nat.RecursiveIn O f) (hg:Nat.RecursiveIn O g):Nat.RecursiveIn O fun a => if (c a=0) then (f a) else (g a) := by
+    have exists_index_for_f:∃ c:ℕ, eval O c = f := by exact exists_code_nat.mp hf
+    have exists_index_for_g:∃ c:ℕ, eval O c = g := by exact exists_code_nat.mp hg
+    rcases exists_index_for_f with ⟨index_f,index_f_is_f⟩
+    rcases exists_index_for_g with ⟨index_g,index_g_is_g⟩
+
+    have main2:(fun a => if (c a=0) then (f a) else (g a)) = fun a => Nat.pair (if c a=0 then (index_f) else (index_g)) a >>= eval₁ O := by
+      funext xs
+      cases Classical.em (c xs = 0) with
+      | inl h =>
+        simp only [h, ↓reduceIte, Part.coe_some, Part.bind_eq_bind, Part.bind_some, eval₁, Nat.unpair_pair]
+        exact congrFun (_root_.id (Eq.symm index_f_is_f)) xs
+      | inr h =>
+        simp only [h, ↓reduceIte, Part.coe_some, Part.bind_eq_bind, Part.bind_some, eval₁, Nat.unpair_pair]
+        exact congrFun (_root_.id (Eq.symm index_g_is_g)) xs
+    rw [main2]
+
+
+    apply Nat.RecursiveIn.evalRecInO'
+    apply Nat.RecursiveIn.someTotal
+
+    rw [Nat.RecursiveIn.pair']
+
+    apply Nat.RecursiveIn.pair
+    · simp only [Part.coe_some]
+      apply Nat.RecursiveIn.ifz1
+      exact hc
+    exact id
